PMapHelperLemmas.v
@@ -1,0 +1,13 @@
+From MyProject Require Import SmtExpr.
+From MyProject Require Import CrProgramState.
+
+Transparent lookup_ctrl.
+Lemma commute_lookup_eval_ctrl:
+  forall c f s,
+  lookup_ctrl (eval_sym_state s f) c =
+  eval_smt_arith (lookup_ctrl s c) f.
+Proof.
+  intros.
+  apply PMap.gmap.
+Qed.
+Global Opaque lookup_ctrl.
